theories/L2_5_box/awndEval.v
@@ -33,10 +33,10 @@ Inductive awndEval : Term -> Term -> Prop :=
             awndEval (TLetIn nm dfn bod) (instantiate dfn 0 bod)
      (* Case argument must be in Canonical form *)
      (* np is the number of parameters of the datatype *)
-| aCase: forall (ml: inductive * nat * list nat) (s mch:Term)
-                 (args brs ts:Terms) (n arty:nat),
+| aCase: forall (ml: inductive * nat) (s mch:Term)
+                 (args ts:Terms) (brs:Defs) (n arty:nat),
             canonicalP mch = Some (n, args, arty) ->
-            tskipn (snd (fst ml)) args = Some ts ->
+            tskipn (snd ml) args = Some ts ->
             whCaseStep n ts brs = Some s ->
             awndEval (TCase ml mch brs) s
 | aFix: forall (dts:Defs) (m:nat) (arg:Term) (args:Terms)
@@ -60,13 +60,14 @@ Inductive awndEval : Term -> Term -> Prop :=
               awndEval d1 d2 ->
               awndEval (TLetIn nm d1 bod) (TLetIn nm d2 bod)
 | aCaseArg:
-    forall (ml:inductive * nat * list nat) (mch can:Term) (brs:Terms),
+    forall (ml:inductive * nat) (mch can:Term) (brs:Defs),
               awndEval mch can ->
               awndEval (TCase ml mch brs) (TCase ml can brs)
+                       (*************
 | aCaseBrs:
-    forall (ml:inductive * nat * list nat) (mch:Term) (brs brs':Terms),
-              awndEvals brs brs' ->
+    forall (ml:inductive * nat (mch:Term) (brs:Defs),
               awndEval (TCase ml mch brs) (TCase ml mch brs')
+******************)
 with awndEvals : Terms -> Terms -> Prop :=
      | aaHd: forall (t r:Term) (ts:Terms), 
                awndEval t r ->
