theories/L2_5_box/stripWndCommute.v
@@ -17,3 +17,162 @@ Require Import L2_5.compile.
 Definition L2Term := L2.compile.Term.
 Definition L2Terms := L2.compile.Terms.
 Definition L2Defs := L2.compile.Defs.
+
+
+Lemma TApp_mkApp_step_lem:
+  forall fn fn' arg args,
+    TApp fn arg args = mkApp fn' (tcons arg args) -> fn = fn'.
+Proof.
+  destruct fn'; cbn; intros; cbn; try myInjection H; try reflexivity.
+  injection H. intros.
+  assert (j:= f_equal tlength H0). cbn in j.
+  rewrite tlength_tappend in j. cbn in j. omega.
+Qed.
+
+Lemma mkApp_TApp_step_lem:
+  forall fn fn' arg args, ~ isApp fn ->
+    fn = fn' -> TApp fn arg args = mkApp fn' (tcons arg args).
+Proof.
+  destruct fn; intros; subst; cbn; intros; cbn; try reflexivity.
+  elim H. exists fn1, fn2, t. reflexivity.
+Qed.
+
+(***************
+Lemma TConst_strip_inv:
+  forall nm r, TConst nm = strip r ->
+               (r = L2.compile.TConst nm) \/ (L2.term.isCase r).
+Proof.
+  destruct r; intros; try discriminate.
+  - myInjection H. left. reflexivity.
+  - right. exists p, r, d. reflexivity.
+Qed.
+
+
+Lemma Lookup_stripEnv_inv:
+  forall p s sec, Lookup s (stripEnv p) sec ->
+              exists u, Lookup s p u /\ L2EC_EC u = sec.
+Proof.
+  induction p; intros.
+  - inversion H.
+  - destruct a, (string_dec s s0).
+    + subst s. cbn in H.
+      pose proof (LHit s0 (stripEnv p) (L2EC_EC e)).
+      pose proof (Lookup_single_valued H H0). subst sec.
+      exists e. intuition.
+    + cbn in H. inversion_Clear H.
+      * intuition.
+      * specialize (IHp s _ H6). destruct IHp as [u [j1u j2u]].
+        exists u. intuition.
+Qed.
+***********************)
+
+(************
+Theorem L2_5wndEval_sound_for_L2wndEval:
+  forall L2_5p,
+  (forall L2_5t L2_5s, wndEval L2_5p L2_5t L2_5s ->
+  forall p, L2_5p = stripEnv p ->
+  forall t, L2_5t = strip t ->
+            exists s, L2.wndEval.wndEval p t s /\ strip s = L2_5s) /\
+  (forall L2_5t L2_5s, wndEvals L2_5p L2_5t L2_5s ->
+  forall p, L2_5p = stripEnv p ->
+  forall t, L2_5t = strips t ->
+            exists s, L2.wndEval.wndEvals p t s /\ strips s = L2_5s).
+Proof.
+  intros L2_5p.
+  apply (@wndEvalEvals_ind L2_5p
+   (fun (L2_5t L2_5s: Term) (prf: wndEval L2_5p L2_5t L2_5s) =>
+    forall p: L2Env, L2_5p = stripEnv p ->
+    forall t: compile.L2Term, L2_5t = strip t ->
+    exists s: L2.compile.Term, L2.wndEval.wndEval p t s /\ strip s = L2_5s)
+   (fun (L2_5t L2_5s: Terms) (prf: wndEvals L2_5p L2_5t L2_5s) =>
+    forall p: L2Env, L2_5p = stripEnv p ->
+    forall t: compile.L2Terms, L2_5t = strips t ->
+    exists s: L2.compile.Terms, L2.wndEval.wndEvals p t s /\
+                                  strips s = L2_5s));
+    intros.
+  - unfold LookupDfn in l.
+    pose proof (Const_strip_inv _ H0) as k. destruct k.
+    + subst. destruct (Lookup_stripEnv_inv _ _ _ l) as [x [j1x j2x]].
+      destruct x; cbn in j2x.
+      * myInjection j2x. exists l0. intuition.
+      * discriminate.
+    + subst. destruct (Lookup_stripEnv_inv _ _ _ l) as [x [j1x j2x]].
+      destruct H1 as [x0 [x1 [x2 jx]]]. destruct x.
+      *  HERE
+      subst. discriminate.
+  - destruct (App_strip_inv _ H0) as [x0 [x1 [x2 [j1x [j2x [j3x j4x]]]]]].
+    subst. clear H0.
+    destruct (Lam_strip_inv _ j2x) as [y0 [y1 [j1y j2y]]].
+    subst. rewrite <- whBetaStep_hom. exists (L2.term.whBetaStep y1 x1 x2).
+    intuition.
+  - destruct (LetIn_strip_inv _ H0) as [x0 [x1 [x2 [j0x [j1x j2x]]]]].
+    subst. rewrite <- (proj1 instantiate_hom).
+    exists (L2.term.instantiate x0 0 x2). intuition.
+  - destruct (Case_strip_inv _ H0) as [x0 [x1 [j0x [j1x [j2x j3x]]]]].
+    clear H0. subst.
+    rewrite <- canonicalP_hom in e.
+    case_eq (L2.term.canonicalP x1); intros; rewrite H in e; try discriminate.
+    + destruct p0 as [[z0 z1] z2]. cbn in e. myInjection e.
+      destruct ml. cbn in e0.
+      rewrite <- tskipn_hom in e0.
+      case_eq (L2.term.tskipn n0 z1); intros; rewrite H0 in e0;
+      try discriminate.
+      * { cbn in e0. myInjection e0.
+          rewrite <- whCaseStep_hom in e1; try discriminate.
+          case_eq (L2.term.whCaseStep n t j0x); intros; rewrite H1 in e1;
+          try discriminate.
+          - cbn in e1. myInjection e1. exists t0. intuition.
+            econstructor; try eassumption. }
+  - destruct (App_strip_inv _ H0) as [x0 [x1 [x2 [j1x [j2x [j3x j4x]]]]]].
+    subst. clear H0.
+    destruct (Fix_strip_inv _ j2x) as [y0 [j0y j1y]]; intros. subst. clear j2x.
+    rewrite <- dnthBody_hom in e.
+    case_eq (compile.dnthBody m y0); intros; rewrite H in e; try discriminate.
+    + destruct p0. cbn in e. myInjection e. rewrite <- tcons_hom.
+      rewrite pre_whFixStep_hom.
+      exists (L2.term.pre_whFixStep t y0 (L2.compile.tcons x1 x2)).
+      intuition. apply (L2.wndEval.sFix p y0 m x1 x2 H ).
+      rewrite tlength_hom in l. assumption.
+  - destruct (Cast_strip_inv _ H0) as [x0 [x1 [j0x j1x]]]. subst.
+    exists x0. intuition.
+  - destruct (Prf_strip_inv _ H0) as [x0 [j0 j1]]. subst.
+    exists x0. intuition.
+  - destruct (App_strip_inv _ H1) as [x0 [x1 [x2 [j1x [j2x [j3x j4x]]]]]].
+    subst. rewrite <- tcons_hom.
+    destruct (H p eq_refl x0 eq_refl) as [y0 [j0y j1y]].
+    subst. rewrite <- mkApp_hom.
+    exists (L2.term.mkApp y0 (L2.compile.tcons x1 x2)). intuition.
+  - destruct (App_strip_inv _ H1) as [x0 [x1 [x2 [j1x [j2x [j3x j4x]]]]]].
+    subst. clear H1.
+    destruct (H p eq_refl (L2.compile.tcons x1 x2) eq_refl) as
+        [y [j0y j1y]]. clear H.
+    rewrite <- j1y in w. 
+    inversion_Clear j0y.
+    + rewrite tcons_hom in j1y. myInjection j1y.
+      rewrite <- (TApp_hom x0 r x2). exists (L2.compile.TApp x0 r x2).
+      intuition.
+    + rewrite tcons_hom in j1y. myInjection j1y.
+      rewrite <- (TApp_hom x0 x1 ss). exists (L2.compile.TApp x0 x1 ss).
+      intuition.
+  - destruct (LetIn_strip_inv _ H1) as [x0 [x1 [x2 [j0x [j1x j2x]]]]].
+    subst. clear H1.
+    specialize (H p eq_refl x0 eq_refl).
+    destruct H as [y [j0y j1y]]. subst. rewrite <- (TLetIn_hom nm y x1).
+    exists (L2.compile.TLetIn nm y x1 x2). intuition.
+  - destruct (Case_strip_inv _ H1) as [x0 [x1 [j0x [j1x [j2x j3x]]]]].
+    clear H1. subst.
+    specialize (H p eq_refl x1 eq_refl).
+    destruct H as [y [j0y j1y]]. subst. rewrite <- (TCase_hom nl x0 y).
+    exists (L2.compile.TCase nl x0 y j0x). intuition.
+  - destruct (tcons_strip_inv _ H1) as [x0 [x1 [j0x [j1x j2x]]]]. subst.
+    specialize (H p eq_refl x0 eq_refl).
+    destruct H as [y [j0y j1y]]. subst.
+    rewrite <- tcons_hom. exists (L2.compile.tcons y x1). intuition.
+  - destruct (tcons_strip_inv _ H1) as [x0 [x1 [j0x [j1x j2x]]]]. subst.
+    specialize (H p eq_refl x1 eq_refl).
+    destruct H as [y [j0y j1y]]. subst.
+    rewrite <- tcons_hom. exists (L2.compile.tcons x0 y). intuition.
+Qed.
+Print Assumptions L2_5wndEval_sound_for_L2wndEval.
+
+********************)
