theories/L4_deBruijn/L3_to_L4.v
@@ -85,14 +85,13 @@ Section TermTranslation.
     Variable trans : N -> L3t.Term -> exp.
     Definition trans_args (k : N) (t : L3t.Terms) : exps :=
       map_terms (trans k) t.
-    Fixpoint trans_brs ind ann k n l :=
+    Fixpoint trans_brs ind k n l :=
       match l with
-      | L3t.tnil => brnil_e
-      | L3t.tcons t ts =>
-        let nargs := (List.nth (N.to_nat n) ann 0%nat)%nat in
-        let '(names, t') := (strip_lam nargs (trans k t)) in
+      | L3t.dnil => brnil_e
+      | L3t.dcons na t nargs ts =>
+        let '(names, t') := strip_lam nargs (trans k t) in
         brcons_e (ind,n) (N.of_nat nargs, names) t'
-                 (trans_brs ind ann k (n + 1)%N ts)
+                 (trans_brs ind k (n + 1)%N ts)
       end.
     Fixpoint trans_fixes k l :=
       match l with
@@ -119,10 +118,10 @@ Section TermTranslation.
     | L3t.TInd i => (* Erase *) erased_exp
     | L3t.TConstruct ind c args =>
       let args' := trans_args trans k args in
-        Con_e (dcon_of_con ind c) args'
+      Con_e (dcon_of_con ind c) args'
     | L3t.TCase ann t brs =>
-      let '(ind, pars, args) := ann in
-      let brs' := trans_brs trans ind args k 0%N brs in
+      let '(ind, pars) := ann in
+      let brs' := trans_brs trans ind k 0%N brs in
       Match_e (trans k t) (N.of_nat pars) brs'
     | L3t.TFix d n =>
       let len := L3t.dlength d in
